abstract definitions

examples/std/fibo.v
@@ -4,6 +4,86 @@ From monae Require Import preamble hierarchy monad_lib monad_model.
 
 Set Implicit Arguments.
 
+Local Open Scope do_notation.
+Local Open Scope monae_scope.
+
+Section with_cache.
+Variable res : eqType.
+Definition cache := nat -> option res.
+Variable M : stateRunMonad cache idfun.
+Variable f : nat -> res.
+
+Definition update n v : M unit :=
+  do c <- get; let c' x := if x == n then Some v else c x in put c'.
+
+Definition lookup_or_compute n (m : M res) :=
+  do c <- get;
+  if c n is Some x then Ret x else
+  do x <- m; do _ <- update n x; Ret x.
+
+Definition f_trunc k n := if n < k then Some (f n) else None.
+
+Definition goodcache k c := c = f_trunc k.
+
+Definition R {X} k1 k2 (s : M X) (n : (idfun : monad) X) : Type :=
+  forall c, goodcache k1 c ->
+            (runStateT s c).1 = n /\ goodcache k2 (runStateT s c).2.
+
+Lemma Rget k : R k k get (f_trunc k).
+Proof.
+move=> c Hc.
+by rewrite runStateTget.
+Qed.
+
+Lemma Rret k A (a : A) : R k k (Ret a) a.
+Proof.
+move=> c Hc.
+by rewrite runStateTret.
+Qed.
+
+Lemma Rupdate k : R k k.+1 (update k (f k)) tt.
+Proof.
+move=> c Hc.
+rewrite /update runStateTbind runStateTget bindretf runStateTput /=.
+split => //.
+apply: boolp.funext => x.
+rewrite Hc /f_trunc ltnS.
+by case: ltngtP => // ->.
+Qed.
+
+Lemma Rbind k1 k2 k3 A B (m : M A) m' :
+  R k1 k2 m m' -> forall (g : A -> M B) g',
+      (R k2 k3 (g m') (g' m')) ->
+      R k1 k3 (m >>= g) (m' >>= g').
+Proof.
+move=> Rmm' g g' Rgg' c Hc.
+rewrite runStateTbind.
+case: (Rmm' _ Hc).
+case: (runStateT m c) => n2 c2 /= -> /[dup] Hc2 ->.
+rewrite bindretf /=.
+case: (Rgg' _ Hc2).
+rewrite Hc2.
+by move ->.
+Qed.
+
+Lemma Rlookup_or_compute k n (m : M res) :
+  (k <= n -> R k n m (f n)) ->
+  R k (maxn k n.+1) (lookup_or_compute n m) (f n).
+Proof.
+rewrite /lookup_or_compute => Rmm' /=.
+have -> : f n = Ret (f_trunc k) >> Ret (f n) :> (idfun : monad) _ by [].
+apply: Rbind; first exact: Rget.
+rewrite /f_trunc /= /NId /=.
+case: (ltnP k n.+1) => nk; last exact: Rret.
+have -> : f n = Ret (f n) >>= fun x => Ret tt >> Ret x
+        :> (idfun : monad) _ by [].
+exact/(Rbind (Rmm' nk))/Rbind/Rret/Rupdate.
+Qed.
+End with_cache.
+
+Section fibo_with_cache.
+Variable M : stateRunMonad (cache nat) idfun.
+
 Fixpoint fibo n :=
   match n with
   | 0 => 0
@@ -11,23 +91,8 @@ Fixpoint fibo n :=
   | (m.+1 as n).+1 => fibo m + fibo n
   end.
 
-Definition cache := nat -> option nat.
-
-Section with_cache.
-Variable M : stateRunMonad cache idfun.
-Local Open Scope do_notation.
-Local Open Scope monae_scope.
-
-Definition update n v : M unit :=
-  do c <- get; let c' x := if x == n then Some v else c x in put c'.
-
-Definition lookup_or_compute n (m : M nat) :=
-  do c <- get;
-  if c n is Some x then Ret x else
-  do x <- m; do _ <- update n x; Ret x.
-
 Fixpoint fibo_memo n : M nat :=
-  lookup_or_compute n
+  lookup_or_compute M n
     match n with
     | 0 => Ret 0
     | (0 as n).+1 =>
@@ -40,71 +105,8 @@ Fixpoint fibo_memo n : M nat :=
         Ret (x+y)
     end.
 
-Definition fibo_trunc k n := if n < k then Some (fibo n) else None.
-
-Definition goodcache k c := c = fibo_trunc k.
-
-Definition fibocache k :=
-  {c : cache | goodcache k c}.
-
-Definition R {X} k1 k2 (s : M X) (n : (idfun : monad) X) : Type :=
-  forall c, goodcache k1 c ->
-            (runStateT s c).1 = n /\ goodcache k2 (runStateT s c).2.
-
-Lemma Rget k : R k k get (fibo_trunc k).
-Proof.
-move=> c Hc.
-by rewrite runStateTget.
-Qed.
-
-Lemma Rret k A (a : A) : R k k (Ret a) a.
-Proof.
-move=> c Hc.
-by rewrite runStateTret.
-Qed.
-
-Lemma Rupdate k : R k k.+1 (update k (fibo k)) tt.
-Proof.
-move=> c Hc.
-rewrite /update runStateTbind runStateTget bindretf runStateTput /=.
-split => //.
-apply: boolp.funext => x.
-rewrite Hc /fibo_trunc ltnS.
-by case: ltngtP => // ->.
-Qed.
-
-Lemma Rbind k1 k2 k3 A B (m : M A) m' :
-  R k1 k2 m m' -> forall (f : A -> M B) f',
-      (R k2 k3 (f m') (f' m')) ->
-      R k1 k3 (m >>= f) (m' >>= f').
-Proof.
-move=> Rmm' f f' Rff' c Hc.
-rewrite runStateTbind.
-case: (Rmm' _ Hc).
-case: (runStateT m c) => n2 c2 /= -> /[dup] Hc2 ->.
-rewrite bindretf /=.
-case: (Rff' _ Hc2).
-rewrite Hc2.
-by move ->.
-Qed.
-
-Lemma Rlookup_or_compute k n (m : M nat) :
-  (k <= n -> R k n m (fibo n)) ->
-  R k (maxn k n.+1) (lookup_or_compute n m) (fibo n).
-Proof.
-rewrite /lookup_or_compute => Rmm' /=.
-have -> : fibo n = Ret (fibo_trunc k) >> Ret (fibo n)
-        :> (idfun : monad) nat by [].
-apply: Rbind; first exact: Rget.
-rewrite /fibo_trunc /= /NId /=.
-case: (ltnP k n.+1) => nk; last exact: Rret.
-have -> : fibo n = Ret (fibo n) >>= fun x => Ret tt >> Ret x
-        :> (idfun : monad) nat by [].
-exact/(Rbind (Rmm' nk))/Rbind/Rret/Rupdate.
-Qed.
-
-Lemma cacheok : forall n k,
-    R k (maxn k n.+1) (fibo_memo n) (fibo n).
+Lemma fibo_memo_ok : forall n k,
+    R M fibo k (maxn k n.+1) (fibo_memo n) (fibo n).
 Proof.
 elim/ltn_ind => -[|n] IH k;
 rewrite [fibo_memo _]/=;
@@ -124,31 +126,67 @@ rewrite (_ : maxn _ _ = n.+2); last by lia.
 exact: Rret.
 Qed.
 
-(*
-About Fix.
-
-Lemma well_founded_ltn : well_founded (fun x y => x < y).
-Proof. move=> x. Search Acc.
-
-Definition ltn_rec A :
-*)
-
-Variable F : forall N : monad, forall n, (forall k, k < n -> N nat) -> N nat. 
-Let fixF (n : nat) : nat := ltn_ind (F idfun) n.
-Let Fmemo := fun n f => lookup_or_compute n (F M n f).
-Let fixFmemo := ltn_ind Fmemo.
-
-Lemma fixFmemo_ok : forall n k,
-    R k (maxn k n.+1) (fixFmemo n) (fixF n).
-Proof.
-rewrite /fixFmemo /Fmemo /fixF /=.
-elim/ltn_ind => -[|n] IH k.
-Abort.
-
-End with_cache.
-
 Fixpoint fibo' n :=
   match n with
   | 0 => (0, 0.+1)
   | m.+1 => let (a,b) := fibo' m in (b, a+b)
   end.
+End fibo_with_cache.
+
+Section Fixn.
+Variable T : Type.
+Variable F : forall n, (forall k, k < n -> T) -> T. 
+Definition Fixn := 
+  Fix Wf_nat.lt_wf (fun=> T)
+    (fun x f => F x (fun y (yx : y < x) => f y (ltP yx))).
+Lemma Fixn_eq :
+  (forall x (f g : forall y, y < x -> T),
+      (forall y (p : y < x), f y p = g y p) -> F x f = F x g) ->
+  forall x, Fixn x = F x (fun y _ => Fixn y).
+Proof.
+move=> IH.
+apply: Fix_eq => x f g H.
+congr F.
+apply: boolp.functional_extensionality_dep => y.
+apply: boolp.functional_extensionality_dep => yx.
+exact: H.
+Qed.
+End Fixn.
+
+Section fix_with_cache.
+Variable res : eqType.
+Variable M : stateRunMonad (cache res) idfun.
+
+Variable F : forall N : monad, forall n, (forall k, k < n -> N res) -> N res. 
+Let fixF := Fixn (F idfun).
+Let Fmemo := fun n f => lookup_or_compute M n (F M n f).
+Let fixFmemo := Fixn Fmemo.
+
+Hypothesis Funif :
+  forall (N : monad) (x : nat) (f g : forall y : nat, y < x -> N res),
+    (forall (y : nat) (p : y < x), f y p = g y p) -> F N x f = F N x g.
+
+Hypothesis Fpure :
+  forall n c, runStateT (Fixn (F M) n) c = (Fixn (F idfun) n, c).
+
+Lemma fixFmemo_ok : forall n k,
+    R M fixF k (maxn k n.+1) (fixFmemo n) (fixF n).
+Proof.
+rewrite /fixFmemo /Fmemo /fixF /=.
+elim/ltn_ind => -[|n] IH k.
+  rewrite Fixn_eq; last first.
+    move=> x f g H.
+    congr lookup_or_compute.
+    exact: Funif.
+  apply: Rlookup_or_compute.
+  rewrite leqn0 => /eqP ->.
+  rewrite (_ : F M 0 _ = F M 0 (fun y _ => Fixn (F M) y)); last exact: Funif.
+  rewrite -Fixn_eq; last exact: Funif.
+  move=> c Hc. by rewrite Fpure.
+rewrite Fixn_eq; last first.
+  move=> x f g H.
+  by rewrite (Funif _ _ _ g).
+apply: Rlookup_or_compute => kn1.
+Abort.
+
+End fix_with_cache.
